commity

HeapInsert.dfy
@@ -1,8 +1,91 @@
-include "CCPR191-HeapSort-complete-30Dec18.dfy"
+// include "CCPR191-HeapSort-complete-30Dec18.dfy"
 
-method HeapInsert(a: array<int>, heapsize: nat, x: int)
+method {:verify false} parent(index: nat) returns (p: int) 
+{
+	p := (index - 1) / 2;
+}
+predicate AncestorIndex(i: nat, j: nat) decreases j-i 
+{ 
+	i == j || (j > 2*i && ((AncestorIndex(2*i+1, j) || AncestorIndex(2*i+2, j))))
+}
+
+predicate hp(q: seq<int>, length: nat)
+	requires length <= |q|
+{
+	forall i,j :: 0 <= i < length && 0 <= j < length && AncestorIndex(i, j) ==> q[i] >= q[j]
+}
+
+method {:verify false} swap (heap: array<int>, x: nat, y: nat) 
+	modifies heap
+{
+	var temp := heap[x];
+	heap[x] := heap[y];
+	heap[y] := temp;
+}
+
+method {:verify true} HeapInsert(a: array<int>, heapsize: nat, x: int)
 	requires heapsize < a.Length
 	requires hp(a[..], heapsize)
 	ensures hp(a[..], heapsize+1)
 	ensures multiset(a[..heapsize+1]) == multiset(old(a[..heapsize])+[x])
 	modifies a
+{
+	// BottomInsertLemma(a ,heapsize, x);
+	var newHeapsize := BottomInsert(a, heapsize, x);
+	HeapInsert1(a, newHeapsize, x, old(a[..heapsize]));	
+}
+method {:verify true} BottomInsert(a: array<int>, heapsize0: nat, x: int) returns (heapsize: nat)
+	requires heapsize0 < a.Length
+	requires hp(a[..], heapsize0)
+	ensures heapsize <= a.Length
+	ensures multiset(a[..heapsize+1]) == multiset(old(a[..heapsize])+[x])
+	ensures a[heapsize-1] == x
+{
+	Lemma1(a, heapsize0+1, x);
+	a[heapsize0] := x;
+	heapsize := heapsize0 + 1;
+}
+
+lemma Lemma1 (a: array<int>, heapsize: nat, x: int)
+	requires heapsize-1 < a.Length
+	requires hp(a[..], heapsize-1)
+	ensures heapsize == heapsize
+{}
+
+method {:verify true} HeapInsert1(a: array<int>, heapsize: nat, x: int, ghost oldHeap: seq<int>)
+	requires heapsize <= a.Length
+	requires hp(a[..], heapsize-1)
+	requires a[heapsize-1] == x
+	ensures hp(a[..], heapsize)
+	ensures multiset(a[..heapsize]) == multiset(oldHeap[..]+[x])
+	modifies a
+{
+	var current := heapsize; 
+	var parentIndex := parent(current);
+	while (parentIndex >= 0 && a[current] > a[parentIndex]) { 
+		swap(a, current, parentIndex); 
+		current := parent(current); 
+		parentIndex := parent(current);
+	}
+}
+
+
+lemma {:verify true} BottomInsertLemma(a: array<int>, heapsize: nat, x: int)
+	requires heapsize < a.Length
+	requires hp(a[..], heapsize)
+	
+	ensures multiset(a[..heapsize+1]) == multiset(old(a[..heapsize])+[x])
+{}
+
+method Main() {
+	var a := new int[8];
+	a[0] := 6;
+	a[1] := 4;
+	a[2] := 5;
+	a[3] := 3;
+	a[4] := 2;
+	a[5] := 0;
+	a[6] := 1;
+	HeapInsert(a, 7, 8);
+	print a[..];
+}
